Tools/DeclNames.lean
@@ -92,7 +92,9 @@ import Grass.Process.Weave.Lens
 import Grass.Process.Weave.Mixin
 import Grass.Resource.Algebra
 import Grass.Resource.Axis
+import Grass.Refinement.Presentation
 import Grass.Semantics.Execution
+import Grass.Semantics.Behavior
 import Grass.Semantics.Observation
 import Grass.Semantics.SpecProcess
 import Grass.Specification.Boundary
